DeBruijnSSA/BinSyntax/Rewrite/Region/Compose.lean
@@ -1,6 +1,6 @@
 import DeBruijnSSA.BinSyntax.Rewrite.Region.Compose.Seq
 import DeBruijnSSA.BinSyntax.Rewrite.Region.Compose.Product
 import DeBruijnSSA.BinSyntax.Rewrite.Region.Compose.Sum
-import DeBruijnSSA.BinSyntax.Rewrite.Region.Compose.Structural
+import DeBruijnSSA.BinSyntax.Rewrite.Region.Structural
 import DeBruijnSSA.BinSyntax.Rewrite.Region.Compose.Elgot
 import DeBruijnSSA.BinSyntax.Rewrite.Region.Compose.Completeness
